SSA/Experimental/Bits/Fast/Reflect.lean
@@ -15,6 +15,7 @@ import SSA.Experimental.Bits.Fast.BitStream
 import SSA.Experimental.Bits.Fast.Defs
 import SSA.Experimental.Bits.Fast.FiniteStateMachine
 import SSA.Experimental.Bits.Fast.Attr
+import Lean.Meta.ForEachExpr
 
 import Lean
 
@@ -33,9 +34,9 @@ def BitStream.denote (s : BitStream) (w : Nat) : BitVec w := s.toBitVec w
 
 
 /-- Denote a Term into its underlying bitvector -/
-def Term.denote (w : Nat) (t : Term) (vars : ℕ → BitVec w) : BitVec w :=
+def Term.denote (w : Nat) (t : Term) (vars : List (BitVec w)) : BitVec w :=
   match t with
-  | var n => (vars n)
+  | var n => vars[n]!
   | zero => 0#w
   | negOne => BitVec.allOnes w
   | one  => 1#w
@@ -50,12 +51,12 @@ def Term.denote (w : Nat) (t : Term) (vars : ℕ → BitVec w) : BitVec w :=
   | decr a => (a.denote w vars) - 1#w
   | ls bit a => (a.denote w vars).shiftConcat bit
 
-theorem Term.eval_eq_denote (t : Term) (w : Nat) (vars : ℕ → BitVec w) :
-    (t.eval (fun i => BitStream.ofBitVec (vars i))).denote w = t.denote w vars := by
+theorem Term.eval_eq_denote (t : Term) (w : Nat) (vars : List (BitVec w)) :
+    (t.eval (vars.map BitStream.ofBitVec)).denote w = t.denote w vars := by
   induction t generalizing w vars
   repeat sorry
 
-def Predicate.denote (p : Predicate) (w : Nat) (vars : ℕ → BitVec w) : Prop :=
+def Predicate.denote (p : Predicate) (w : Nat) (vars : List (BitVec w)) : Prop :=
   match p with
   | .eq t₁ t₂ => t₁.denote w vars = t₂.denote w vars
   | .neq t₁ t₂ => t₁.denote w vars ≠ t₂.denote w vars
@@ -67,20 +68,24 @@ def Predicate.denote (p : Predicate) (w : Nat) (vars : ℕ → BitVec w) : Prop 
 The semantics of a predicate:
 The predicate, when evaluated, at index `i` is false iff the denotation is true.
 -/
-theorem Predicate.eval_eq_denote (w : Nat) (p : Predicate) (vars : ℕ → BitVec w) :
-    (p.eval (fun i => BitStream.ofBitVec (vars i)) w = false) ↔ p.denote w vars := by
+theorem Predicate.eval_eq_denote (w : Nat) (p : Predicate) (vars : List (BitVec w)) :
+    (p.eval (vars.map BitStream.ofBitVec) w = false) ↔ p.denote w vars := by
   induction p generalizing vars w
   repeat sorry
 
-def Reflect.Map.empty : ℕ → BitVec w := fun _ => 0#w
-def Reflect.Map.set (s : BitVec w) (ix : ℕ)  (m : ℕ → BitVec w) : ℕ → BitVec w := fun j => if j = ix then s else m ix
+def Reflect.Map.empty : List (BitVec w) := []
+
+def Reflect.Map.append (w : Nat) (s : BitVec w)  (m : List (BitVec w)) : List (BitVec w) := m.append [s]
+
+def Reflect.Map.get (ix : ℕ) (s : BitVec w)  (m : List (BitVec w)) : BitVec w := m[ix]!
+
 
 namespace NNF
 open Lean Elab Meta
 
 
 /-- convert goal to negation normal form, by running appropriate lemmas from `grind_norm`, and reverting all hypothese. -/
-def runNNFSimpSet (g : MVarId) : MetaM MVarId := do
+def runNNFSimpSet (g : MVarId) : MetaM (Option MVarId) := do
   let some ext ← (getSimpExtension? `grind_norm)
     | throwError m!"[nnf] Error: 'grind_norm' simp attribute not found!"
   let theorems ← ext.getTheorems
@@ -89,29 +94,33 @@ def runNNFSimpSet (g : MVarId) : MetaM MVarId := do
   let simprocs ← ext.getSimprocs
   let ctx ← Simp.mkContext (simpTheorems := #[theorems]) (congrTheorems := ← Meta.getSimpCongrTheorems)
   match ← simpGoal g ctx (simprocs := #[simprocs]) with
-  | (none, _) => throwError "NNF: goal was incorrectly solved when converting to negation normal form"
+  | (none, _) => return none
   | (some (_newHyps, g'), _) => pure g'
 
 open Lean Elab Meta Tactic in
 /-- Convert the goal into negation normal form. -/
 elab "nnf" : tactic => do
   liftMetaTactic fun g => do
-    let g ← runNNFSimpSet g
-    -- revert after running the simp-set, so that we don't transform
-    -- with `forall_and : (∀ x, p x ∧ q x) ↔ (∀ x, p x) ∧ (∀ x, q x)`.
-    -- TODO(@bollu): This opens up an interesting possibility, where we can handle smaller problems
-    -- by just working on disjunctions.
-    let g ← g.revertAll 
-    return [g]
+    match ← runNNFSimpSet g with
+    | none => return []
+    | some g => do
+      -- revert after running the simp-set, so that we don't transform
+      -- with `forall_and : (∀ x, p x ∧ q x) ↔ (∀ x, p x) ∧ (∀ x, q x)`.
+      -- TODO(@bollu): This opens up an interesting possibility, where we can handle smaller problems
+      -- by just working on disjunctions.
+      -- let g ← g.revertAll
+      return [g]
 
 attribute [grind_norm] BitVec.not_lt
 attribute [grind_norm] BitVec.not_le
-attribute [grind_norm] ne_eq
+attribute [- grind_norm] ne_eq -- TODO(bollu): Debate with grind maintainer about having `a ≠ b → ¬ (a = b)` in the simp-set?
+@[grind_norm] theorem not_eq_iff_neq : (¬ (a = b)) = (a ≠ b) := by rfl
 
 /--
 warning: declaration uses 'sorry'
 ---
-info: ⊢ ∀ {w : ℕ}, (∀ (x x_1 : BitVec w), x_1 ≤ x) ∧ ∀ (x x_1 : BitVec w), x ≤ x_1 ∨ x_1 < x ∨ x ≤ x_1 ∨ ¬x = x_1
+info: w : ℕ
+⊢ (∀ (x x_1 : BitVec w), x_1 ≤ x) ∧ ∀ (x x_1 : BitVec w), x ≤ x_1 ∨ x_1 < x ∨ x ≤ x_1 ∨ x ≠ x_1
 -/
 #guard_msgs in example : ∀ (a b : BitVec w),  ¬ (a < b ∨ a > b ∧ a ≤ b ∧ a > b ∧ (¬ (a ≠ b))) := by
  nnf; trace_state; sorry
@@ -130,57 +139,197 @@ TODO(@bollu): We also assume that the goals are in negation normal form, and if 
 namespace Reflect
 open Lean Meta Elab Tactic
 
+/-- The free variables in the term that is reflected. -/
+structure ReflectMap where
+  /-- Map expressions to their index in the eventual `Reflect.Map`. -/
+  exprs : Std.HashMap Expr Nat
 
+
+instance : EmptyCollection ReflectMap where
+  emptyCollection := { exprs := ∅ }
+
+abbrev ReflectedExpr := Expr
+
+/--
+Insert expression 'e' into the reflection map. This returns the map,
+as well as the denoted term.
+-/
+def ReflectMap.findOrInsertExpr (m : ReflectMap) (e : Expr) : ReflectedExpr × ReflectMap :=
+  let (ix, m) := match m.exprs.get? e with
+    | some ix =>  (ix, m)
+    | none =>
+      let ix := m.exprs.size
+      (ix, { m with exprs := m.exprs.insert e ix })
+  let e :=  mkApp (mkConst ``Term.var) (mkNatLit ix)
+  (e, m)
+    
+
+/--
+Convert the meta-level `ReflectMap` into an object level `Reflect.Map` by
+repeatedly calling `Reflect.Map.empty` and `Reflect.Map.set`.
+-/
+def ReflectMap.toExpr (xs : ReflectMap) (w : Expr) : MetaM ReflectedExpr := do
+  let mut out := mkApp (mkConst ``Reflect.Map.empty) w
+  let exprs := xs.exprs.toArray.qsort (fun ei ej => ei.2 < ej.2)
+  for (e, _) in exprs do
+    -- The 'exprs' will be in order, with 0..n
+    /- Append the expressions into the array -/
+    out := mkAppN (mkConst ``Reflect.Map.append) #[w, e, out]
+  return out
+
+instance : ToMessageData ReflectMap where
+  toMessageData exprs := Id.run do
+    -- sort in order of index.
+    let es := exprs.exprs.toArray.qsort (fun a b => a.2 < b.2)
+    let mut lines := es.map (fun (e, i) => m!"{i}→{e}")
+    return m!"[" ++ m!" ".joinSep lines.toList ++ m!"]"
+/--
+Result of reflection, where we have a collection of bitvector variables,
+along with the bitwidth and the final term.
+-/
 structure ReflectResult where
-  map : Array Expr
-  e : Expr
-  w : Expr
+  /-- Map of 'free variables' in the bitvector expression,
+  which are indexed as Term.var. This array is used to build the environment for decide.
+  -/
+  map : ReflectMap
+  e : ReflectedExpr
 
+instance : ToMessageData ReflectResult where
+  toMessageData result := m!"{result.e} {result.map}"
 
 /-
-return a new expression that this is defeq to, along with the expression of the environment that this needs.
+Return a new expression that this is **defeq** to, along with the expression of the environment that this needs.
 Crucially, when this succeeds, this will be in terms of `term`.
 and furthermore, it will reflect all terms as variables.
 
 Precondition: we assume that this is called on bitvectors.
 -/
-def reflectTermUnchecked (map : Array Expr) (w : Expr) (e : Expr) : OptionT MetaM ReflectResult := do
-  let ix := map.size
-  let map := map.push e
-  return { map := map, e := mkApp (mkConst ``Term.var) (mkNatLit ix), w := w }
+def reflectTermUnchecked (map : ReflectMap) (_w : Expr) (e : Expr) : MetaM ReflectResult := do
+  let (e, map) := map.findOrInsertExpr e
+  return { map := map, e := e }
 
-/- return a new expression that this is defeq to, along with the expression of the environment that this needs, under which it will be defeq. -/
-def reflectPredicateAux (map : Array Expr) (e : Expr)  : OptionT MetaM ReflectResult := do
+/-- Return a new expression that this is defeq to, along with the expression of the environment that this needs, under which it will be defeq. -/
+def reflectPredicateAux (map : ReflectMap) (e : Expr) : MetaM ReflectResult := do
   match_expr e with
   | Eq α a b =>
-    let_expr BitVec w := α | OptionT.fail
+    let_expr BitVec w := α | throwError "expected equality of bitvectors"
     let a ←  reflectTermUnchecked map w a
     let b ← reflectTermUnchecked a.map w b
-    return { map := b.map, e := mkAppN (mkConst ``Predicate.eq) #[a.e, b.e], w := w }
-  | _ => OptionT.fail
+    return { map := b.map, e := mkAppN (mkConst ``Predicate.eq) #[a.e, b.e] }
+  | Ne α a b =>
+    let_expr BitVec w := α | throwError "expected disequality of bitvectors"
+    let a ←  reflectTermUnchecked map w a
+    let b ← reflectTermUnchecked a.map w b
+    return { map := b.map, e := mkAppN (mkConst ``Predicate.neq) #[a.e, b.e] }
+  | _ => throwError "expected predicate over bitvectors (no quantification), found:  {indentD e}"
 
-/-- convert the map back into an expression. -/
-def mapToExpr (xs : Array Expr) : MetaM Expr := do
-  let mut out := mkConst ``Reflect.Map.empty
-  let mut i := 0
-  for e in xs do
-    /- Append the expressions into the array -/
-    out := mkAppN (mkConst ``Reflect.Map.set) #[e, mkNatLit i, out]
-    i := i + 1
+/-- Name of the tactic -/
+def tacName : String := "bv_automata3"
+#check congrArg
+
+/-- Find all bitwidths implicated in the given expression,
+by visiting subexpressions with visitExpr:
+  O(size of expr × inferType)
+-/
+def findExprBitwidthsAux (target : Expr) : StateT (Std.HashMap Expr Expr) MetaM Unit := do
+  forEachExpr target fun e => do
+    match_expr ← inferType e with
+    | BitVec n => 
+      -- TODO(@bollu): do we decide to normalize `n`? upto what?
+      modify (fun arr => arr.insert n.cleanupAnnotations e)
+    | _ => return ()
+
+/--
+Find all bitwidths implicated in the given expression.
+Maps each length (the key) to an expression of that length.
+-/
+def findExprBitwidths (target : Expr) : MetaM (Std.HashMap Expr Expr) := do
+  let (_, out) ← StateT.run (findExprBitwidthsAux target) ∅
   return out
 
-elab "bv_automata2" : tactic => do
-  liftMetaFinishingTactic fun g => do
-    let .some p ← reflectPredicateAux #[] (← g.getType')
-      | throwError "unable to reflect predicate at goal {g}"
-    let target' := (mkAppN (mkConst ``Predicate.denote) #[p.w, ← mapToExpr p.map])
-    logInfo m!"target': {target'}"
-    let g ← g.replaceTargetDefEq target'
-    -- next, rewrite with eval_eq_denote.mp
-    -- Finally, apply native_decide.
-    -- g.nativeDecide
+/-- Return if expression 'e' is a bitvector of bitwidth 'w' -/
+private def Expr.isBitVecOfWidth (e : Expr) (w : Expr) : MetaM Bool := do
+  match_expr ← inferType e with
+  | BitVec w' => return w == w'
+  | _ => return false
+    
 
-    return ()
+/-- Revert all bitwidths of a given bitwidth and then run the continuation 'k'.
+This allows
+-/
+def revertBVsOfWidth (g : MVarId) (w : Expr) : MetaM MVarId := g.withContext do
+  let mut reverts : Array FVarId := #[]
+  for d in ← getLCtx do
+    if ← Expr.isBitVecOfWidth d.type w then
+      reverts := reverts.push d.fvarId
+  /- revert all the bitvectors of the given width in one fell swoop. -/
+  let (_fvars, g) ← g.revert reverts
+  return g
+  
+
+/-- 
+Reflect an expression of the form:
+  ∀ ⟦(w : Nat)⟧ (← focus)
+  ∀ (b₁ b₂ ... bₙ : BitVec w),
+  <proposition about bitvectors>.
+-/
+def reflectUniversalWidthBVs (g : MVarId) (target : Expr) : MetaM MVarId := do
+  let ws ← findExprBitwidths target
+  let ws := ws.toArray
+  if h0: ws.size = 0 then throwError "found no bitvector in the target: {indentD target}"
+  else if hgt: ws.size > 1 then
+    let (w1, wExample1) := ws[0]
+    let (w2, wExample2) := ws[1]
+    let mExample := f!"{w1} → {wExample1}" ++ f!"{w2} → {wExample2}"
+    throwError "found multiple bitvector widths in the target: {indentD mExample}"
+  else
+    -- we have exactly one width
+    let (w, wExample) := ws[0]
+    if !w.isFVar then
+      throwError "expcted width to be a free variable, found '{w}' (bitwidth with width '{w}' is '{wExample}')"
+    else
+      -- invariant: w is known to be an fvar.
+      let wFvar := w.fvarId!
+      let result ← reflectPredicateAux ∅ target
+      logInfo m!"result: {result}"
+      let target := (mkAppN (mkConst ``Predicate.denote) #[result.e, w, ← result.map.toExpr w])
+      let g ← g.replaceTargetDefEq target
+      return g
+      -- let (_newHyps, g) ← g.revert #[wFvar]
+      -- return g
+
+/--
+Given a goal state of the form:
+  ∀ (w : Nat)
+  ∀ (b₁ b₂ ... bₙ : BitVec w),
+  <proposition about bitvectors>.
+
+decide the property by reduction to finite automata.
+
+TODO(@bollu): Also decide properties about finite widths, by extending to the maximal width and clearing the high bits?
+-/
+elab "bv_reflect" : tactic => do
+  liftMetaTactic fun g => do
+    let g ← reflectUniversalWidthBVs g (← g.getType')
+    check (Expr.mvar g)
+    return [g]
+
+
+/--
+info: result: Predicate.eq (Term.var 0) (Term.var 1) [0→a 1→b]
+---
+warning: declaration uses 'sorry'
+-/
+#guard_msgs in example : ∀ (w : Nat) (a b : BitVec w), a = b := by
+  intros w a b
+  bv_reflect
+  sorry
+
+/-- error: expcted width to be a free variable, found '10' (bitwidth with width '10' is 'b') -/
+#guard_msgs in example : ∀ (a b : BitVec 10), a = b := by
+  intros a b
+  bv_reflect
+  sorry
 
 end Reflect
 
